Tables/Data/Array/Pairwise.lean
@@ -11,6 +11,22 @@ theorem Pairwise.filter {α} {R : α → α → Prop} {a : Array α} (p : α →
   rw [Pairwise, Array.toList_filter]
   exact List.Pairwise.filter p h
 
+theorem pairwise_map {α β} {R : β → β → Prop} {f : α → β} {a : Array α} :
+    (a.map f).Pairwise R ↔ a.Pairwise (fun a b => R (f a) (f b)) := by
+  rw [Pairwise, Array.toList_map]
+  exact List.pairwise_map
+
+theorem pairwise_attach {α} {R : α → α → Prop} {a : Array α}  :
+    a.attach.Pairwise (fun a b => R a.val b.val) ↔ a.Pairwise R := by
+  simp only [Pairwise, attach, attachWith, List.attachWith, List.pairwise_pmap]
+  rw [List.pairwise_iff_getElem, List.pairwise_iff_getElem]
+  simp
+
+theorem pairwise_unattach {α} {R : α → α → Prop} {p : α → Prop} {a : Array { a : α // p a }} :
+    a.unattach.Pairwise R ↔ a.Pairwise (fun a b => R a.val b.val) := by
+  simp [Pairwise, Array.toList_unattach]
+  rw [List.unattach, List.pairwise_map]
+
 end Array
 
 end
